start making the TSSA again

SSA/WellTypedFramework.lean
@@ -66,45 +66,6 @@ def trdTriple [Goedel β] {k₁ k₂ k₃ : UserType β} : ⟦k₁.triple k₂ k
 end UserType
 
 
-structure UserData {β : Type} [Goedel β] where
-  type : UserType β
-  value : toType type
-
-/-- `TypeData` is a `Type` used to represent a potentially unknown `UserType`,
-usually of a variable in the context.
-for the purposes of type inference of `SSA`. `any` means that the `UserType`
-is completely unknown, `unused` means that a variable is unused, `pair` means that
-it is known that the type is a pair, but the elements of the pair are not necessarily
-known and so on. -/
-inductive  TypeData (β : Type) : Type
-  | some : β → TypeData β
-  | unit : TypeData β
-  | pair : TypeData β → TypeData β → TypeData β
-  | triple : TypeData β → TypeData β → TypeData β → TypeData β
-  | region : TypeData β → TypeData β → TypeData β
-  | any : TypeData β
-  | unused : TypeData β -- Or bound
-
-@[coe]
-def UserType.toTypeData [Goedel β] : UserType β → TypeData β
-  | UserType.base t => TypeData.some t
-  | UserType.unit => TypeData.unit
-  | UserType.pair k₁ k₂ => TypeData.pair (UserType.toTypeData k₁) (UserType.toTypeData k₂)
-  | UserType.triple k₁ k₂ k₃ => TypeData.triple (UserType.toTypeData k₁) (UserType.toTypeData k₂)
-    (UserType.toTypeData k₃)
-  | UserType.region k₁ k₂ => TypeData.region (UserType.toTypeData k₁) (UserType.toTypeData k₂)
-
-variable {β : Type} [instDecidableEqBaseType : DecidableEq β] [instGoedel : Goedel β]
-instance : Coe (UserType β) (TypeData β) := ⟨UserType.toTypeData⟩
-
-def TypeData.toUserType : TypeData β → Option (UserType β)
-  | TypeData.some t => do return UserType.base t
-  | TypeData.unit => do return UserType.unit
-  | TypeData.pair k₁ k₂ => do UserType.pair (← k₁.toUserType) (← k₂.toUserType)
-  | TypeData.triple k₁ k₂ k₃ => do UserType.triple (← k₁.toUserType) (← k₂.toUserType) (← k₃.toUserType)
-  | TypeData.region k₁ k₂ => do UserType.region (← k₁.toUserType) (← k₂.toUserType)
-  | TypeData.any => none
-  | TypeData.unused => none
 
 /-- Typeclass for a user semantics of `Op`, with base type `β`.
     The type β has to implement the `Goedel` typeclass, mapping into `Lean` types.
@@ -117,240 +78,35 @@ def TypeData.toUserType : TypeData β → Option (UserType β)
     * `eval` gives the actual evaluation semantics of the operation, by defining a function for
       every operation `o : Op` of type `toType (argUserType o) → (toType (rgnDom o) → toType (rgnCod o)) → toType (outUserType o)`.
 -/
-class TypedUserSemantics (Op : Type) (β : Type) [Goedel β] where
+class OperationTypes (Op : Type) (β : Type) where
   argUserType : Op → UserType β
   rgnDom : Op → UserType β
   rgnCod : Op → UserType β
   outUserType : Op → UserType β
+
+class TypedUserSemantics (Op : Type) (β : Type) [Goedel β] extends OperationTypes Op β where
   eval : ∀ (o : Op), toType (argUserType o) → (toType (rgnDom o) →
-    Option (toType (rgnCod o))) → Option (toType (outUserType o))
+    toType (rgnCod o)) → toType (outUserType o)
 
-@[simp]
-def TypeData.toType : TypeData β → Type
-  | TypeData.some t => Goedel.toType t
-  | TypeData.unit => Unit
-  | TypeData.pair t₁ t₂ => (TypeData.toType  t₁) × (TypeData.toType t₂)
-  | TypeData.triple t₁ t₂ t₃ => (TypeData.toType t₁) × (TypeData.toType t₂) × (TypeData.toType t₃)
-  | TypeData.region t₁ t₂ => (TypeData.toType t₁) → Option (TypeData.toType t₂)
-  | TypeData.any => Σ (k : UserType β), ⟦k⟧
-  | TypeData.unused => Unit
+inductive Context (α : Type) : Type
+  | empty : Context α
+  | cons : Var → α → Context α → Context α
 
-instance : Goedel (TypeData β) where
-  toType := TypeData.toType
+inductive Context.Var {α : Type} : Context α → α → Type
+  | first {Γ : Context α} (v : SSA.Var) (a : α) :
+      Context.Var (Context.cons v a Γ) a
+  | next {Γ : Context α} :
+      Context.Var Γ a → Context.Var (Context.cons v' a' Γ) a
 
-theorem TypeDataToTypeEqUserTypeToType (a : UserType β) :
-  toType a = TypeData.toType a.toTypeData :=
-  by
-    induction a <;>
-      (simp [Goedel.toType, TypeData.toType, UserType.toType] at * <;> aesop)
+instance {α : Type} : EmptyCollection (Context α) :=
+  ⟨Context.empty⟩
 
-def Context (α : Type) : Type :=
-  AList (fun _ : Var => α)
-
-instance {α : Type} : EmptyCollection (Context α) := by
-  dsimp [Context]; infer_instance
-
-def Context.pmapCore {α β : Type} (f : α → Option β) :
-    List (Σ _ : Var, α) → Option (List (Σ _ : Var, β))
-  | [] => some []
-  | (⟨v, a⟩ :: l) => do
-    let b ← f a
-    let l' ← Context.pmapCore f l
-    some (⟨v, b⟩ :: l')
-
-theorem Context.pmapCore_keys {α β : Type} (f : α → Option β) :
-    ∀ (l : List (Σ _ : Var, α)),
-    ∀ l' ∈ (Context.pmapCore f l), l'.keys = l.keys
-  | [] => by simp [Context.pmapCore]
-  | (a::l) => by
-    rintro l'
-    simp only [Context.pmapCore, List.keys_cons]
-    cases h : f a.2
-    . simp [bind]
-    . cases h' : pmapCore f l
-      . simp [bind]
-      . simp only [Option.some_bind, Option.mem_def, Option.some.injEq, bind]
-        rintro rfl
-        rw [← Context.pmapCore_keys f _ _ h']
-        simp
-
-def Context.pmap {α β : Type} (f : α → Option β) (l : Context α) : Option (Context β) := by
-  cases h : Context.pmapCore f l.1 with
-  | none => exact none
-  | some l' => exact some ⟨l', by rw [List.NodupKeys, Context.pmapCore_keys _ _ _ h]; exact l.2⟩
-
-
-@[simp]
-def SSAIndex.ieval (β : Type) : SSAIndex → Type
-  | .TERMINATOR => TypeData β
-  | .EXPR => TypeData β
-  | .REGION => TypeData β
-  | .STMT => List Var
-
-def SSAIndex.ieval.any {β : Type} : (i : SSAIndex) → i.ieval β
-  | .TERMINATOR => TypeData.any
-  | .EXPR => TypeData.any
-  | .REGION => TypeData.region TypeData.any TypeData.any
-  | .STMT => []
-
-/-- A Monad used to keep track of a typing context for variables during `inferType`. -/
-abbrev TypeContextM (β : Type)
-  : Type → Type := StateT (Context (TypeData β)) Option
-
--- Lean gets very picky here and wants to get all instances passed explicit to be sure they're the same
-def getVars : TypeContextM β (Var → TypeData β) := do
-  let al := (← StateT.get)
-  return (fun v => match al.lookup v with
-    | some t => t
-    | none => TypeData.unused)
-
-def getVarType (v : Var) : TypeContextM β (TypeData β) :=
-  do return (← getVars) v
-
-def updateType (v : Var) (t : TypeData β) : TypeContextM β Unit := do
-  StateT.modifyGet (fun s => ((), s.insert v t))
-
-/-- assign a variable. Fails if the variable is not unused to start with -/
-def assignVar (v : Var) (t : TypeData β) : TypeContextM β Unit := do
-  let k ← getVarType v
-  match k with
-  | .unused => updateType v t
-  | _ => failure
-
-/-- Does not change the state. Fails if impossible to unify.
-TypeData is a meet semilattice with top element `unused`.  -/
-def unify : (t₁ t₂ : TypeData β) → TypeContextM β (TypeData β)
-  | .unused, k => return k
-  | k, .unused => return k
-  | .any, k => return k
-  | k, .any => return k
-  | .some k₁, .some k₂ => do
-    if k₁ = k₂
-    then return .some k₁
-    else failure
-  | .pair k₁ k₂, .pair t₁ t₂ => do
-    return .pair (← unify k₁ t₁) (← unify k₂ t₂)
-  | .triple k₁ k₂ k₃, .triple t₁ t₂ t₃ => do
-    return .triple (← unify k₁ t₁) (← unify k₂ t₂) (← unify k₃ t₃)
-  | .region k₁ k₂, .region t₁ t₂ => do
-    return .region (← unify k₁ t₁) (← unify k₂ t₂)
-  | .unit, .unit => return .unit
-  | _, _ => failure
-
-def unifyVar (v : Var) (t : TypeData β) : TypeContextM β  (TypeData β) := do
-  let k ← getVarType v
-  let k' ← unify k t
-  updateType v k'
-  return k'
-
-@[simp]
-def assignAny (t : Var → TypeData β) (v : Var) : TypeContextM β Unit :=
-  match t v with
-  | .unused => assignVar v .any
-  | _ => failure
-
-def unassignVars (l : List Var) : TypeContextM β Unit := do
-  l.forM (fun v => updateType v .unused)
-
-/-- Given an expected type, tries to infer the type of an expression.
-The state consists of the expected type of any free variables, and this state is
-updated based on the new information.
-* If `STMT` then return a list of names of variables used in the `STMT`.
-Change the state to include types for all variables assigned in the `STMT`.
-Ignore expected type, because this is a list of variables anyway.
-Fails if assigned variable is not `unused` in initial state.
-* If `TERMINATOR` then change state for free variables, but not bound ones.
-Return the type of the returned variable. Fails when bound variable is not `unused` initially
-* If `EXPR`, then return type of expression, and do not change the type of bound
-variables, only free variables.
-* If `REGION` then as for `EXPR`  -/
--- @chris: the type signature should be `SSA Op i → TypeContextM (Context β)`?
-def inferTypeCore {Op : Type}  [TUS : TypedUserSemantics Op β] :
-    {i : SSAIndex} → SSA Op i →
-    (i.ieval β)
-    → TypeContextM β (i.ieval β)
-  | _,  .assign lhs rhs rest, _ => do
-    let k ← inferTypeCore rhs (← getVarType lhs)
-    assignVar lhs k
-    let l ← inferTypeCore rest []
-    return lhs :: l
-  | _, .nop, _ => return []
-  | _, .ret s v, k => do
-    let l ← inferTypeCore s []
-    let k' ← unifyVar v k
-    unassignVars l
-    return k'
-  | _, .unit, k => do
-    unify .unit k
-  | _, .pair fst snd, k => do
-    unify (.pair (← getVarType fst) (← getVarType snd)) k
-  | _, .triple fst snd trd, k => do
-    unify (.triple (← getVarType fst) (← getVarType snd) (← getVarType trd)) k
-  | _,  .op o arg r, _ => do
-    let _ ← unifyVar arg (TUS.argUserType o)
-    let dom := TUS.rgnDom o
-    let cod := TUS.rgnCod o
-    let _ ← inferTypeCore r (.region dom cod)
-    return (TypedUserSemantics.outUserType o).toTypeData
-  | _, .var v, k => unifyVar v k
-  | _, .rgnvar v, k => do
-    unifyVar v (← unify k (.region TypeData.any TypeData.any))
-  | _, .rgn0, k => do
-    unify k (.region TypeData.unit TypeData.unit)
-  | _, .rgn arg body, k => do
-    match ← unify k (.region TypeData.any TypeData.any) with
-    | .region dom cod => do
-      let dom ← unifyVar arg dom
-      let cod ← inferTypeCore body cod
-      unassignVars [arg]
-      return .region dom cod
-    | _ => failure
-
-def inferType {Op : Type} [TypedUserSemantics Op β]
-    {i : SSAIndex} (e : SSA Op i) :
-    Option ((i.ieval β) × Context (UserType β)) := do
-  let k ← inferTypeCore (β := β) e (SSAIndex.ieval.any i) ∅
-  return (k.1, ← k.2.pmap TypeData.toUserType)
-
-/-- A typed evaluation environment, given a typing context `c`, an `EnvC c`
-contains semantics for all of the variables in the `Context`, `c`. -/
-def EnvC (c : Context (UserType β)) :=
-  ∀ (v : Var), (c.lookup v).elim Unit UserType.toType
-
---instance {β : Type} [Goedel β] {c : Context (UserType β)}: EmptyCollection (EnvC c) := by
---  sorry
-
-variable (β)
-
-/-- An untyped value - the semantics of many programs will return a `UVal` -/
-def UVal := Σ (k : UserType β), k.toType
-
-/-- An untyped evaluation environment, contains optional semantics for all variables. -/
-def EnvU : Type :=
-  Var → Option (UVal β)
-
-instance {β : Type} [Goedel β] : EmptyCollection (EnvU β) where
-  emptyCollection := (fun _ => none)
-
-variable {β}
-
-@[simp]
-def EnvC.toEnvU {c : Context (UserType β)} (e : EnvC c) : EnvU β := by
-  dsimp [EnvC] at *
-  intro v
-  have ev := e v
-  revert ev
-  cases c.lookup v
-  . exact fun _ => none
-  . exact fun x => return ⟨_, x⟩
-
-@[simp]
-def EnvU.set : EnvU β → Var → UVal β → EnvU β
-  | e, v, u => fun v' => if v = v' then u else e v'
+def EnvC [Goedel β] (c : Context (UserType β)) :=
+  ∀ (a : UserType β), c.Var a → ⟦a⟧
 
 @[simp]
 def SSAIndex.teval (Op : Type) (β : Type) [Goedel β]
-    [TypedUserSemantics Op β] : SSAIndex → Type
+    [OperationTypes Op β] : SSAIndex → Type
 | .STMT => Option (EnvU β)
 | .TERMINATOR => Option (UVal β)
 | .EXPR => Option (UVal β)
